more compile bitvec progress

lib/CompileBitVec.v
@@ -20,6 +20,8 @@ Set Universe Polymorphism.
 Require Import SMTCoq.SMTCoq.
 
 Import BVList.BITVECTOR_LIST.
+Require Import Coq.Lists.List.
+Import ListNotations.
 
 Section CompileBitVec.
 
@@ -30,7 +32,7 @@ Section CompileBitVec.
 
   Definition conv_arr := @fmap_arity FirstOrderBitVec.sig BV.sig conv_sort.
 
-  (* pulled from Clement Pit-Claudel's blog: https://plv.csail.mit.edu/blog/computing-with-opaque-proofs.html#computing-with-opaque-proofs *)
+  (* Inspired by Clement Pit-Claudel's blog post: https://plv.csail.mit.edu/blog/computing-with-opaque-proofs.html#computing-with-opaque-proofs *)
   Definition comp_eq_N {m n: N} (opaque_eq: m = n) : m = n :=
     match N.eq_dec m n with
     | left transparent_eq => transparent_eq
@@ -42,10 +44,7 @@ Section CompileBitVec.
     | left transparent_eq => transparent_eq
     | right _ => opaque_eq
     end.
-
-  Print N.eq_dec.
   
-
   Definition trans_inj_add : forall n n' : nat, N.of_nat (n + n') = (N.of_nat n + N.of_nat n')%N 
     := fun n n' => comp_eq_N (Nat2N.inj_add n n').
 
@@ -61,6 +60,9 @@ Section CompileBitVec.
   (* use t2l to convert bs to a list and cast the length of t2l to w *)
   Definition conv_n_tuple (w: nat) (bs: n_tuple bool w) : bitvector (N.of_nat w) :=
     eq_rect _ (fun n => bitvector (N.of_nat n)) (of_bits (t2l bs)) _ (trans_t2l_len _ bs).
+
+  Definition conv_bitvector {n} (x: bitvector n) : n_tuple bool (N.to_nat n) :=
+    eq_rect _ _ (l2t (bits x)) _ (comp_eq_nat (bits_size x)).
 
 
   Local Obligation Tactic := intros.
@@ -91,10 +93,33 @@ Section CompileBitVec.
   Definition conv_rel {arr } (r: sig_rels FirstOrderBitVec.sig arr) : sig_rels sig (conv_arr arr) := 
     match r with end.
 
-  Equations conv_mv {srt} (v: FirstOrderBitVec.mod_sorts srt) : BV.mod_sorts (conv_sort srt) := 
-  {
-    @conv_mv (Bits n) bv := conv_n_tuple _ bv;
-  }.
+  Definition conv_mv {srt} (v: FirstOrderBitVec.mod_sorts srt) : BV.mod_sorts (conv_sort srt) := 
+    match srt as srt' return FirstOrderBitVec.mod_sorts srt' -> BV.mod_sorts (conv_sort srt') with 
+    | Bits n => fun v' => conv_n_tuple _ v'
+    end v.
+
+  (* Unfortunately this does not typecheck *)
+  (* Lemma conv_mv_bitvector: 
+    forall {n} bv, 
+      @conv_mv (Bits n) (conv_bitvector bv) = bv.  *)
+
+  Require Import Coq.PArith.Pnat.
+
+  Lemma conv_mv_bitvector: 
+    forall {n} bs bs' bv, 
+      @conv_mv (Bits n) bs = bv -> 
+      conv_bitvector bv = bs' -> 
+      bs ~= bs'.
+  Proof.
+    induction n; intros; simpl in *.
+    - destruct bs, bs'; eapply JMeq_refl.
+    - admit.
+      (* destruct bs.
+      subst.
+      unfold conv_n_tuple.
+      erewrite SuccNat2Pos.id_succ in bs'. *)
+  Admitted.
+
 
   Program Definition conv_functor : @theory_functor FirstOrderBitVec.sig BV.sig FirstOrderBitVec.fm_model BV.fm_model := {|
     fmap_sorts := @conv_sort;
@@ -102,8 +127,6 @@ Section CompileBitVec.
     fmap_rels := @conv_rel;
     fmap_mv := @conv_mv;
   |}.
-
-  (* Notation fmap_ctx := (@fmap_ctx n2z_func). *)
 
   Notation fmap_ctx' := (fmap_ctx _ _ _ _ conv_functor).
 
@@ -118,13 +141,12 @@ Section CompileBitVec.
     conv_fun_arrs (Slice n hi lo) (x ::: _) := _;
   }.
   Next Obligation.
-  exact (x ::: y ::: hnil).
+    exact (x ::: y ::: hnil).
   Defined.
   Next Obligation.
-  exact (x ::: hnil).
+    exact (x ::: hnil).
   Defined.
 
-  Transparent conv_fun_arrs.
 
   Definition conv_rel_arrs {c arr} (rel: FirstOrderBitVec.rels arr) (args: HList.t (fun srt' : FirstOrderBitVec.sorts => FirstOrder.tm sig (fmap_ctx' c) (conv_sort srt')) arr) 
     : HList.t (FirstOrder.tm sig (fmap_ctx' c)) (conv_arr arr) := 
@@ -132,21 +154,164 @@ Section CompileBitVec.
 
   Program Definition conv_forall_op {c} {srt: sig_sorts FirstOrderBitVec.sig} (f: FirstOrder.fm sig (fmap_ctx' (Snoc _ c srt))) : FirstOrder.fm sig (fmap_ctx' (Snoc _ c srt)) := f.
 
-  Program Definition conv_wf : functor_wf _ _ _ _ conv_functor (@conv_fun_arrs) (@conv_rel_arrs) (@conv_forall_op) := {|
-    interp_tm_inj := _;
+  Lemma fmap_tm_inj: 
+    forall {srt c} {v: valu _ _ c} 
+      (t t': FirstOrder.tm FirstOrderBitVec.sig c srt), 
+      interp_tm v t = interp_tm v t' <-> 
+      interp_tm
+        (fmap_valu
+          FirstOrderBitVec.sig
+          sig
+          FirstOrderBitVec.fm_model
+          fm_model
+          conv_functor v)
+        (fmap_tm
+          FirstOrderBitVec.sig
+          sig
+          FirstOrderBitVec.fm_model
+          fm_model
+          conv_functor
+          (@conv_fun_arrs) t) =
+      interp_tm
+        (fmap_valu
+          FirstOrderBitVec.sig
+          sig
+          FirstOrderBitVec.fm_model
+          fm_model
+          conv_functor v)
+        (fmap_tm
+          FirstOrderBitVec.sig
+          sig
+          FirstOrderBitVec.fm_model
+          fm_model
+          conv_functor
+          (@conv_fun_arrs) t').
+  Admitted.
+
+  Lemma interp_fmap_fm_equi: 
+    forall {c srt} {v: valu _ _ c}
+      (f: FirstOrder.fm FirstOrderBitVec.sig (Snoc _ c srt)),
+    (forall
+      vA : FirstOrder.mod_sorts
+              FirstOrderBitVec.sig
+              FirstOrderBitVec.fm_model
+              srt,
+    interp_fm
+      (VSnoc sig fm_model
+          (fmap_sorts
+            conv_functor srt)
+          (fmap_ctx' c)
+          (fmap_valu
+            FirstOrderBitVec.sig
+            sig
+            FirstOrderBitVec.fm_model
+            fm_model
+            conv_functor v)
+          (fmap_mv
+            conv_functor srt
+            vA))
+      (fmap_fm
+          FirstOrderBitVec.sig
+          sig
+          FirstOrderBitVec.fm_model
+          fm_model
+          conv_functor
+          (@conv_fun_arrs)
+          (@conv_rel_arrs)
+          (@conv_forall_op) f)) <->
+    (forall
+      vB : FirstOrder.mod_sorts
+              sig fm_model
+              (fmap_sorts
+                conv_functor
+                srt),
+    interp_fm
+      (VSnoc sig fm_model
+          (fmap_sorts
+            conv_functor srt)
+          (fmap_ctx' c)
+          (fmap_valu
+            FirstOrderBitVec.sig
+            sig
+            FirstOrderBitVec.fm_model
+            fm_model
+            conv_functor v)
+          vB)
+      (conv_forall_op
+          (fmap_fm
+            FirstOrderBitVec.sig
+            sig
+            FirstOrderBitVec.fm_model
+            fm_model
+            conv_functor
+            (@conv_fun_arrs)
+            (@conv_rel_arrs)
+            (@conv_forall_op)
+            f))).
+  Proof.
+    intros.
+    unfold conv_forall_op.
+    simpl.
+    dependent induction f; destruct srt; simpl; 
+    autorewrite with fmap_fm;
+    autorewrite with interp_fm.
+    - split; intros; autorewrite with interp_fm in *; trivial.
+    - split; intros; autorewrite with interp_fm in *; trivial.
+      + specialize (H (n_tuple_repeat n false)).
+        auto.
+      + specialize (H (conv_n_tuple _ vA)).
+        auto.
+    - split; intros; autorewrite with fmap_fm in *; autorewrite with interp_fm in *; simpl in *.
+      + 
+        pose (vA := conv_bitvector vB).
+        admit.
+        (* pose proof @conv_mv_bitvector n vA.
+        specialize (H1 vA).
+        
+        specialize (H vA).
+        autorewrite with interp_fm in H.
+        eapply H. *)
+      + specialize (H (conv_n_tuple _ vA)).
+        now autorewrite with interp_fm in *.
+
+    - inversion s.
+    - split; intros.
+      + autorewrite with fmap_fm.
+        autorewrite with interp_fm.
+        (* use conv_bitvector and a correctness lemma here *)
+        admit.
+      + 
+        specialize (H (conv_n_tuple _ vA)).
+        autorewrite with fmap_fm in *.
+        autorewrite with interp_fm in *.
+        eapply H.
+    - split; intros; autorewrite with interp_fm.
+      + admit.
+      + specialize (H (conv_n_tuple _ vA)).
+        autorewrite with interp_fm in H.
+        destruct H; intuition eauto.
+    - split; intros; autorewrite with interp_fm.
+      + admit.
+      + specialize (H (conv_n_tuple _ vA)).
+        autorewrite with interp_fm in H.
+        intuition eauto.
+    - split; intros; autorewrite with interp_fm.
+      + admit.
+      + specialize (H (conv_n_tuple _ vA)).
+        autorewrite with interp_fm in H.
+        intuition eauto.
+    - split; intros; autorewrite with interp_fm.
+      + admit.
+      + specialize (H (conv_n_tuple _ vA)).
+        autorewrite with interp_fm in H.
+        intuition eauto.
+  Admitted.
+
+  Definition conv_wf : functor_wf _ _ _ _ conv_functor (@conv_fun_arrs) (@conv_rel_arrs) (@conv_forall_op) := {|
+    interp_tm_inj := ltac:(intros; eapply fmap_tm_inj);
     fmap_rel_equi := ltac:(intros; inversion r);
-    interp_fmap_forall_equi := _;
+    interp_fmap_forall_equi := ltac:(intros; eapply interp_fmap_fm_equi);
   |}.
-  Next Obligation.
-  Admitted.
-  Next Obligation.
-  unfold conv_forall_op.
-  simpl.
-  dependent induction f; 
-  try now ( 
-    split; intros; autorewrite with interp_fm in *; trivial
-  ).
-  Admitted.
 
   Lemma conv_corr: 
     forall (c : ctx FirstOrderBitVec.sig) (v : valu FirstOrderBitVec.sig FirstOrderBitVec.fm_model c) (f : FirstOrder.fm FirstOrderBitVec.sig c),
